discharge(stlc): infer over build carrier

Lp2lc/Next/STLC/__Infer.lean
@@ -8,16 +8,15 @@ namespace AST
 
 /-- Infers build types for executable terms, recursively resolving runtime references. -/
 def infer [env : BuildEnv]
-    (self : Trm env.ExeF) : RecOpt (Typ env.BuildF)
+    (self : Trm env.BuildF) : RecOpt (Typ env.BuildF)
   | 0 => .outOfFuel
   | fuel + 1 =>
     match self with
     | .val (.lit _) => .yield (some .primitive)
     | .val (.lam body tIn) =>
-      let cIn : Typ env.BuildF := Typ.recarrier tIn
-      let index : env.ExeF.Carrier := by sorry
+      let index : env.BuildF.Carrier := .inr (env.trm2typCtx.inv (.lam body tIn))
       (infer (body index) fuel).map
-        (λ out => out.map (λ tOut => .fn cIn tOut))
+        (λ out => out.map (λ tOut => .fn tIn tOut))
     | .apply fnTerm arg =>
       match infer fnTerm fuel, infer arg fuel with
       | .yield (some (.fn tIn tOut)), .yield (some argTyp) =>
@@ -25,9 +24,13 @@ def infer [env : BuildEnv]
       | .outOfFuel, _ => .outOfFuel
       | _, .outOfFuel => .outOfFuel
       | _, _ => .yield none
-    | .ref receipt =>
-      let original := env.trm2valCtx.get receipt
+    | .ref (.inl receipt) =>
+      let original : Val env.BuildF := mapCarrier (Sum.inl) (env.trm2valCtx.get receipt)
       original.asTrm.infer fuel
+    | .ref (.inr receipt) =>
+      match env.trm2typCtx.get receipt with
+      | .lit _ => .yield (some .primitive)
+      | .lam _ tIn => .yield (some tIn)
 
 /-
 DEFER: GPT is right:
@@ -43,7 +46,7 @@ DEFER: GPT is right:
 -/
 
 def CanInhabit [env : BuildEnv]
-    (self : Trm env.ExeF) (typ : Typ env.BuildF) : Prop :=
+    (self : Trm env.BuildF) (typ : Typ env.BuildF) : Prop :=
   self.infer.isDecidable (λ inferred => inferred ≤ typ)
 
 end AST
@@ -52,6 +55,7 @@ class ProvingBase extends BuildEnv
 
 def Safety [env : ProvingBase]
     (trm : AST.Trm env.ExeF) (typ : AST.Typ env.BuildF) : Prop :=
-  trm.eval.isSemiDecidable (λ value => value.asTrm.CanInhabit typ)
+  trm.eval.isSemiDecidable
+    (λ value => (AST.mapCarrier (Sum.inl) value.asTrm).CanInhabit typ)
 
 end Lp2lc.Next.STLC
